theories/zoo/program_logic/prophet_identifier.v
@@ -1,0 +1,47 @@
+From zoo Require Import
+  prelude.
+From zoo.language Require Import
+  notations.
+From zoo.program_logic Require Export
+  identifier
+  prophet_typed.
+From zoo Require Import
+  options.
+
+Program Definition prophet_identifier := {|
+  prophet_typed_type :=
+    identifier ;
+  prophet_typed_of_val v :=
+    match v with
+    | ValId id =>
+        Some id
+    | _ =>
+        None
+    end ;
+  prophet_typed_to_val id :=
+    #id ;
+|}.
+Solve Obligations of prophet_identifier with
+  try done.
+Next Obligation.
+  naive_solver.
+Qed.
+
+Program Definition prophet_identifier_1 := {|
+  prophet_typed_1_type :=
+    identifier ;
+  prophet_typed_1_of_val v :=
+    match v with
+    | ValId id =>
+        Some id
+    | _ =>
+        None
+    end ;
+  prophet_typed_1_to_val id :=
+    #id ;
+|}.
+Solve Obligations of prophet_identifier_1 with
+  try done.
+Next Obligation.
+  naive_solver.
+Qed.
